formal/inference/heuristics/Symbolic_Regression.thy
@@ -382,6 +382,35 @@ fun put_updates :: "log \<Rightarrow> value list \<Rightarrow> transition \<Righ
       put_updates log values t1 lit ops updated
   )"
 
+(* This works the other way to the regular apply_updates but since there'll only ever be one per register, it's equivalent *)
+primrec apply_updates_redundancy :: "updates \<Rightarrow> datastate \<Rightarrow> registers \<Rightarrow> updates \<Rightarrow> (registers \<times> updates)" where
+  "apply_updates_redundancy [] _ new redundant = (new, redundant)" |
+  "apply_updates_redundancy (h#t) old new redundant = (
+    if old (R (fst h)) = aval (snd h) old then
+      (apply_updates_redundancy t old (new(fst h $:= aval (snd h) old)) (h#redundant))
+    else
+      (apply_updates_redundancy t old (new(fst h $:= aval (snd h) old)) redundant)
+  )"
+
+fun remove_redundant_updates :: "execution \<Rightarrow> iEFSM \<Rightarrow> cfstate \<Rightarrow> registers \<Rightarrow> iEFSM" where
+  "remove_redundant_updates [] e _ _ = e" |
+  "remove_redundant_updates ((label, inputs, outputs)#t) e s r = (
+    let (tid, s', ta) = fthe_elem (ffilter (\<lambda>(_, _, t). apply_outputs (Outputs t) (join_ir inputs r) = map Some outputs) (i_possible_steps e s r label inputs)) in
+    if outgoing_transitions s' e = {||} then
+      let newT = \<lparr>Label = Label ta, Arity = Arity ta, Guard = Guard ta, Outputs = Outputs ta, Updates = []\<rparr> in
+      remove_redundant_updates t (replace_transition e tid newT) s' r
+    else
+      let
+      (updated, redundant) = apply_updates_redundancy (Updates ta) (join_ir inputs r) r [];
+      newT = \<lparr>Label = Label ta, Arity = Arity ta, Guard = Guard ta, Outputs = Outputs ta, Updates = filter (\<lambda>u. u \<notin> set redundant) (Updates ta)\<rparr>
+    in
+      remove_redundant_updates t (replace_transition e tid newT) s' updated
+  )"
+
+primrec remove_redundant_updates_log :: "log \<Rightarrow> iEFSM \<Rightarrow> iEFSM" where
+  "remove_redundant_updates_log [] e = e" |
+  "remove_redundant_updates_log (h#t) e = remove_redundant_updates_log t (remove_redundant_updates h e 0 <>)"
+
 definition historical_infer_output_update_functions :: "log \<Rightarrow> update_modifier" where
   "historical_infer_output_update_functions log t1ID t2ID s new _ old np = (
     let
@@ -403,7 +432,11 @@ definition historical_infer_output_update_functions :: "log \<Rightarrow> update
         Some lit \<Rightarrow> (
           case put_updates log values t1 lit (enumerate 0 output_functions) new of
             None \<Rightarrow> None |
-            Some updated \<Rightarrow> resolve_nondeterminism [] (sorted_list_of_fset (np updated)) old updated null_modifier (\<lambda>a. True) np
+            Some updated \<Rightarrow> (
+              case resolve_nondeterminism [] (sorted_list_of_fset (np updated)) old updated null_modifier (\<lambda>a. True) np of
+                None \<Rightarrow> None |
+                Some new \<Rightarrow> Some (remove_redundant_updates_log log new)
+          )
         )
   )"
 
